Wavelet/Semantics/OpInterp.lean
@@ -19,19 +19,15 @@ instance : Arity Empty where
 inductive RespLabel Op V [Arity Op] where
   | respond (op : Op) (inputs : Vector V (Arity.ι op)) (outputs : Vector V (Arity.ω op))
 
-/-- Base semantics interprets all of the operators in the same LTS
-with potentially shared states.
-
-TODO: The fact that we need two definitions of semantics (`OpInterp`
-and `Semantics`) is a bit unfortunate. Try unify?
--/
-class OpInterp (Op : Type u) (V : Type v) [Arity Op] where
-  S : Type w
-  init : S
-  lts : Lts S (RespLabel Op V)
+def RespLabel.MatchLabel
+  [Arity Op]
+  {V : Type v} : RespLabel Op V → Label Op V m n → Prop
+  | .respond op₁ inputs₁ outputs₁, .yield op₂ inputs₂ outputs₂ =>
+    op₁ = op₂ ∧ inputs₁ ≍ inputs₂ ∧ outputs₁ ≍ outputs₂
+  | _, _ => False
 
 /-- Parallel composition of `sem` and `interp`. -/
-inductive InterpStep
+inductive Lts.InterpStep
   [Arity Op]
   (base : Lts S₁ (Label Op V m n))
   (interp : Lts S₂ (RespLabel Op V)) : Lts (S₁ × S₂) (Label Empty V m n) where
@@ -49,6 +45,36 @@ inductive InterpStep
     interp.Step t (.respond op inputs outputs) t' →
     InterpStep base interp (s, t) .τ (s', t')
 
+/-- Similar to `Interp`, but allowing additional indices in the base LTS. -/
+inductive Lts.IndexedInterpStep
+  [Arity Op] {I}
+  (base : Lts S₁ (I × Label Op V m n))
+  (interp : Lts S₂ (RespLabel Op V)) : Lts (S₁ × S₂) (I × Label Empty V m n) where
+  | step_tau :
+    base.Step s (i, .τ) s' →
+    IndexedInterpStep base interp (s, t) (i, .τ) (s', t)
+  | step_input :
+    base.Step s (i, .input inputVals) s' →
+    IndexedInterpStep base interp (s, t) (i, .input inputVals) (s', t)
+  | step_output :
+    base.Step s (i, .output outputVals) s' →
+    IndexedInterpStep base interp (s, t) (i, .output outputVals) (s', t)
+  | step_yield :
+    base.Step s (i, .yield op inputs outputs) s' →
+    interp.Step t (.respond op inputs outputs) t' →
+    IndexedInterpStep base interp (s, t) (i, .τ) (s', t')
+
+/-- Base semantics interprets all of the operators in the same LTS
+with potentially shared states.
+
+TODO: The fact that we need two definitions of semantics (`OpInterp`
+and `Semantics`) is a bit unfortunate. Try unify?
+-/
+class OpInterp (Op : Type u) (V : Type v) [Arity Op] where
+  S : Type w
+  init : S
+  lts : Lts S (RespLabel Op V)
+
 /-- Fully interpret all operators using a `OpInterp` to get
 a transition system with only input/output/silent events. -/
 def interpret
@@ -59,7 +85,7 @@ def interpret
   := {
     S := sem.S × interp.S,
     init := (sem.init, interp.init),
-    lts := InterpStep sem.lts interp.lts,
+    lts := Lts.InterpStep sem.lts interp.lts,
   }
 
 /-- Deterministic operator set. -/
@@ -71,19 +97,19 @@ def OpInterp.Deterministic
     interp.lts.Step s (.respond op inputs outputs₂) s₂' →
     s₁' = s₂' ∧ outputs₁ = outputs₂
 
-def InterpStep.map_step
+def Lts.Interp.map_step
   [Arity Op] {S S'}
   {lts₁ lts₂ : Lts S (Label Op V m n)}
   {lts' : Lts S' (RespLabel Op V)}
   {s s' : S × S'}
   (hmap : ∀ {s s' l}, lts₁.Step s l s' → lts₂.Step s l s')
-  (hstep : (InterpStep lts₁ lts').Step s l s') :
-    (InterpStep lts₂ lts').Step s l s'
+  (hstep : (Lts.InterpStep lts₁ lts').Step s l s') :
+    (Lts.InterpStep lts₂ lts').Step s l s'
   := by
   cases hstep with
-  | step_tau hstep => exact InterpStep.step_tau (hmap hstep)
-  | step_input hstep => exact InterpStep.step_input (hmap hstep)
-  | step_output hstep => exact InterpStep.step_output (hmap hstep)
-  | step_yield hbase hinterp => exact InterpStep.step_yield (hmap hbase) hinterp
+  | step_tau hstep => exact .step_tau (hmap hstep)
+  | step_input hstep => exact .step_input (hmap hstep)
+  | step_output hstep => exact .step_output (hmap hstep)
+  | step_yield hbase hinterp => exact .step_yield (hmap hbase) hinterp
 
 end Wavelet.Semantics
