Wavelet.lean
@@ -3,5 +3,6 @@ import Wavelet.Seq
 import Wavelet.Dataflow
 import Wavelet.Compile
 
--- TODO: move this to better places
+-- TODO: move these to better places
 import Wavelet.Determinacy
+import Wavelet.Typing
